src/kemedhoc/Impl.KEMEDHOC.Core.Msg2.Aux.fst
@@ -1,0 +1,522 @@
+module Impl.KEMEDHOC.Core.Msg2.Aux
+
+(*LowStar related modules*)
+open Lib.ByteBuffer
+open Lib.IntTypes
+open Lib.Buffer
+
+(*HACL Random lib*)
+open Lib.RandomBuffer.System
+module HACLRandom = Lib.RandomSequence
+
+module B = LowStar.Buffer
+module ST = FStar.HyperStack.ST
+module HS = FStar.HyperStack
+module S = FStar.Seq
+module Seq = Lib.Sequence
+
+(*Specification modules*)
+module Spec = Spec.KEMEDHOC.Core
+
+module FBytes = FStar.Bytes
+
+module SpecCrypto = Spec.KEMEDHOC.CryptoPrimitives
+module SpecParser = Spec.KEMEDHOC.Parser
+module SpecTH = Spec.KEMEDHOC.TranscriptHash
+module SpecKS = Spec.KEMEDHOC.KeySchedule
+
+module SpecEdhocSerd = Spec.EDHOC.Serialization
+
+module TypeEdhoc = TypeHelper.EDHOC
+
+(*EDHOC utilities*)
+open Impl.EDHOC.Utilities
+
+(*KEMEDHOC utilities*)
+open Impl.KEMEDHOC.Types
+open Impl.KEMEDHOC.CryptoPrimitives
+open Impl.KEMEDHOC.KeySchedule
+open Impl.KEMEDHOC.Parser
+open Impl.KEMEDHOC.Ciphertext
+open Impl.KEMEDHOC.TranscriptHash
+open Impl.KEMEDHOC.Core
+open Spec.KEMEDHOC.Base.Definitions
+
+(*-------------- Utilities*)
+inline_for_extraction noextract
+let lbufferOpt_get_value (#len: size_t)
+  (buff: lbufferOpt len)
+  : lbuffer uint8 len
+  = buff.value
+
+/// Disjoint to Context 2
+let handshake_state_m_disjoint_to_context2 (#kcs: supportedKemCipherSuite)
+  (hs: handshake_state_m kcs) (ctx2: context2 kcs)
+  = B.all_disjoint [
+    // handshake_state fields
+    loc hs.suite_i; loc hs.msg1_hash;
+    loc hs.k_xy.is_some; loc hs.k_xy.value;
+    loc hs.k_auth_R;
+    loc hs.k_auth_I.is_some; loc hs.k_auth_I.value;
+    loc hs.th1;
+    loc hs.th2.is_some; loc hs.th2.value;
+    loc hs.th3.is_some; loc hs.th3.value;
+    loc hs.th4.is_some; loc hs.th4.value;
+    loc hs.prk1e;
+    loc hs.prk2e.is_some; loc hs.prk2e.value;
+    loc hs.prk3e2m.is_some; loc hs.prk3e2m.value;
+    loc hs.prk4e3m.is_some; loc hs.prk4e3m.value;
+    loc hs.prk_out.is_some; loc hs.prk_out.value;
+    loc hs.prk_exporter.is_some; loc hs.prk_exporter.value;
+
+    // context 2 fields
+    loc ctx2.c_r; loc ctx2.id_cred_r; loc ctx2.cred_r;
+    loc ctx2.th2
+  ]
+
+/// Disjoint to Plaintext 2
+let handshake_state_m_disjoint_to_p2 (#kcs: supportedKemCipherSuite)
+  (hs: handshake_state_m kcs) (p2: plaintext2 kcs)
+  = B.all_disjoint [
+    // handshake_state fields
+    loc hs.suite_i; loc hs.msg1_hash;
+    loc hs.k_xy.is_some; loc hs.k_xy.value;
+    loc hs.k_auth_R;
+    loc hs.k_auth_I.is_some; loc hs.k_auth_I.value;
+    loc hs.th1;
+    loc hs.th2.is_some; loc hs.th2.value;
+    loc hs.th3.is_some; loc hs.th3.value;
+    loc hs.th4.is_some; loc hs.th4.value;
+    loc hs.prk1e;
+    loc hs.prk2e.is_some; loc hs.prk2e.value;
+    loc hs.prk3e2m.is_some; loc hs.prk3e2m.value;
+    loc hs.prk4e3m.is_some; loc hs.prk4e3m.value;
+    loc hs.prk_out.is_some; loc hs.prk_out.value;
+    loc hs.prk_exporter.is_some; loc hs.prk_exporter.value;
+    loc hs.remote_id_cred.is_some; loc hs.remote_id_cred.value;
+
+    // plaintext 2 fieldds
+    loc p2.c_R; loc p2.id_cred_R;
+    loc p2.cred_R; loc p2.mac2
+  ]
+
+let party_state_disjoint_to_p2 (#kcs: supportedKemCipherSuite)
+  (ps: party_state_m kcs) (p2: plaintext2 kcs)
+  = B.all_disjoint [
+    // party_state fields
+    loc ps.suite; loc (fst ps.static_kem_kp);
+    loc (snd ps.static_kem_kp);
+    loc ps.id_cred;
+    loc ps.eph_kem_priv_key.is_some; loc ps.eph_kem_priv_key.value;
+    loc ps.remote_static_kem_pub_key; loc ps.remote_id_cred;
+
+    // message 2 fields
+    loc p2.c_R; loc p2.id_cred_R;
+    loc p2.cred_R; loc p2.mac2
+  ]
+
+/// Disjoint to Message 2
+let handshake_state_m_disjoint_to_msg2 (#kcs: supportedKemCipherSuite)
+  (hs: handshake_state_m kcs) (msg2: message2 kcs)
+  = B.all_disjoint [
+    // handshake_state fields
+    loc hs.suite_i; loc hs.msg1_hash;
+    loc hs.k_xy.is_some; loc hs.k_xy.value;
+    loc hs.k_auth_R;
+    loc hs.k_auth_I.is_some; loc hs.k_auth_I.value;
+    loc hs.th1;
+    loc hs.th2.is_some; loc hs.th2.value;
+    loc hs.th3.is_some; loc hs.th3.value;
+    loc hs.th4.is_some; loc hs.th4.value;
+    loc hs.prk1e;
+    loc hs.prk2e.is_some; loc hs.prk2e.value;
+    loc hs.prk3e2m.is_some; loc hs.prk3e2m.value;
+    loc hs.prk4e3m.is_some; loc hs.prk4e3m.value;
+    loc hs.prk_out.is_some; loc hs.prk_out.value;
+    loc hs.prk_exporter.is_some; loc hs.prk_exporter.value;
+    loc hs.remote_id_cred.is_some; loc hs.remote_id_cred.value;
+
+    // message 2 fields
+    loc msg2.ct_y; loc msg2.ct_auth_I;
+    loc msg2.c2
+  ]
+
+let party_state_disjoint_to_msg2 (#kcs: supportedKemCipherSuite)
+  (ps: party_state_m kcs) (msg2: message2 kcs)
+  = B.all_disjoint [
+    // party_state fields
+    loc ps.suite; loc (fst ps.static_kem_kp);
+    loc (snd ps.static_kem_kp);
+    loc ps.id_cred;
+    loc ps.eph_kem_priv_key.is_some; loc ps.eph_kem_priv_key.value;
+    loc ps.remote_static_kem_pub_key; loc ps.remote_id_cred;
+
+    // message 2 fields
+    loc msg2.ct_y; loc msg2.ct_auth_I;
+    loc msg2.c2
+  ]
+
+let message2_disjoint_to_p2 (#kcs: supportedKemCipherSuite)
+  (msg2: message2 kcs) (p2: plaintext2 kcs)
+  = B.all_disjoint [
+    // message 2 fieldds
+    loc msg2.ct_y; loc msg2.ct_auth_I;
+    loc msg2.c2;
+
+    // plaintext 2 fields
+    loc p2.c_R; loc p2.id_cred_R;
+    loc p2.cred_R; loc p2.mac2
+  ]
+
+let message2_disjoint_to_msg1 (#kcs: supportedKemCipherSuite)
+  (msg2: message2 kcs) (msg1: message1 kcs)
+  = B.all_disjoint [
+    // message 2 fields
+    loc msg2.ct_y; loc msg2.ct_auth_I;
+    loc msg2.c2;
+
+    // message 1 fields
+    loc msg1.method; loc msg1.suite_i;
+    loc msg1.pk_x; loc msg1.ct_auth_R;
+    loc msg1.c_i; loc msg1.c1
+  ]
+
+
+#push-options "--z3rlimit 40 --max_fuel 4 --max_ifuel 4"
+let responder_construct_msg2_uti (#kcs: supportedKemCipherSuite)
+  (hs: handshake_state_m kcs) (ctx2: context2 kcs) (c2: c2_buff kcs)
+  : ST.Stack c_response
+  (requires fun h0 ->
+    is_valid_handshake_state_m h0 hs
+    /\ is_valid_context2 h0 ctx2
+    /\ live h0 c2
+
+    // Disjointness
+    /\ handshake_state_m_disjoint_to_lbuffer hs c2
+    /\ B.all_disjoint [loc c2; loc ctx2.c_r; loc ctx2.id_cred_r;
+                      loc ctx2.cred_r; loc ctx2.th2; loc hs.th2.value;
+                      loc hs.prk2e.value; loc hs.prk3e2m.value]
+
+    /\ lbufferOpt_is_Some h0 hs.prk3e2m
+  
+  )
+  (ensures fun h0 res h1 ->
+    match res with
+      | TypeEdhoc.CUnsupportedAlgorithmOrInvalidConfig -> modifies0 h0 h1
+      | TypeEdhoc.CSuccess -> (
+        modifies1 c2 h0 h1
+        /\ is_valid_handshake_state_m h1 hs
+        /\ is_valid_context2 h1 ctx2
+      )
+      | _ -> False
+  )
+  = ST.push_frame();
+  (**) let h0 = ST.get () in 
+  // derive MAC2
+  let mac2: mac23_buff kcs = create (size (SpecCrypto.mac23_size kcs)) (u8 0) in
+  (**) let h1 = ST.get () in
+  (**) assert(is_valid_context2 h1 ctx2 /\ live h1 hs.prk3e2m.value /\ live h1 mac2
+        /\ B.all_disjoint [loc hs.prk3e2m.value; loc hs.th2.value ; loc mac2]
+    );
+  // !!! Error in BigOps here. Do not know why
+  expand_mac2 #kcs hs.prk3e2m.value ctx2 mac2;
+  (**) let h2 = ST.get () in
+
+  // construct plaintext2
+  let p2: plaintext2 kcs = {
+    c_R = ctx2.c_r;
+    id_cred_R = ctx2.id_cred_r;
+    cred_R = ctx2.cred_r;
+    mac2 = mac2;
+  } in
+
+  // encrypt plaintext2
+  let res = encrypt_plaintext2 #kcs p2 hs.th2.value hs.prk2e.value c2 in
+  (**) let h3 = ST.get () in
+  (**) assert(res == TypeEdhoc.CSuccess \/ res == TypeEdhoc.CUnsupportedAlgorithmOrInvalidConfig);
+  (**) assert(match res with
+      | TypeEdhoc.CSuccess -> modifies1 c2 h2 h3
+      | TypeEdhoc.CUnsupportedAlgorithmOrInvalidConfig -> modifies0 h2 h3  
+  );
+
+  ST.pop_frame();
+  res
+
+#pop-options
+
+(*----------------- Initiator's side*)
+val initiator_process_msg2_set_up:
+  kcs: supportedKemCipherSuite
+  -> is: party_state_m kcs
+  -> hs: handshake_state_m kcs
+  -> msg2: message2 kcs
+  -> ST.Stack unit
+  (requires fun h0 ->
+    is_valid_handshake_state_m h0 hs
+    /\ is_valid_party_state_m h0 is /\ lbufferOpt_is_Some h0 is.eph_kem_priv_key
+    /\ is_valid_message2 h0 msg2
+
+    // Disjointness
+    /\ handshake_state_m_disjoint_to_party_state hs is
+    /\ handshake_state_m_disjoint_to_msg2 hs msg2
+    /\ party_state_disjoint_to_msg2 is msg2
+  )
+  (ensures fun h0 _ h1 ->
+    let modified_locs = lbufferOpt_loc hs.k_xy |+| lbufferOpt_loc hs.k_auth_I
+              |+| lbufferOpt_loc hs.th2 |+| lbufferOpt_loc hs.prk2e in
+
+    modifies modified_locs h0 h1
+    /\ is_valid_handshake_state_m h1 hs
+    /\ is_valid_party_state_m h1 is
+    /\ is_valid_message2 h1 msg2
+  )
+
+#push-options "--z3rlimit 30 --max_fuel 4 --max_ifuel 4"
+let initiator_process_msg2_set_up kcs is hs msg2
+  = (**) let h0 = ST.get () in
+  // decap ct_y -> k_xy
+  let sk_X = is.eph_kem_priv_key.value in
+  kem_decaps kcs sk_X msg2.ct_y hs.k_xy.value;
+  lbufferOpt_set_Some hs.k_xy; // set Some for k_xy
+  (**) let h1 = ST.get () in
+  (**) assert(modifies (lbufferOpt_loc hs.k_xy) h0 h1);
+
+  // decap ct_auth_I -> k_auth_I
+  let sk_I = snd is.static_kem_kp in
+  kem_decaps kcs sk_I msg2.ct_auth_I hs.k_auth_I.value;
+  lbufferOpt_set_Some hs.k_auth_I; // set Some for k_auth_I
+  (**) let h2 = ST.get () in
+  (**) assert(modifies (lbufferOpt_loc hs.k_xy |+| lbufferOpt_loc hs.k_auth_I) h0 h2);
+
+  // derive TH2
+  compute_th2_pre_hash #kcs msg2.ct_y hs.k_auth_I.value hs.msg1_hash hs.th2.value;
+  lbufferOpt_set_Some hs.th2; // set Some for th2
+  (**) let h3 = ST.get () in
+  (**) assert(modifies (lbufferOpt_loc hs.k_xy |+| lbufferOpt_loc hs.k_auth_I
+              |+| lbufferOpt_loc hs.th2) h0 h3);
+
+  // derive PRK2e
+  extract_prk2e #kcs hs.prk1e hs.th2.value hs.k_xy.value hs.prk2e.value;
+  lbufferOpt_set_Some hs.prk2e; // set Some for prk2e
+  (**) let h4 = ST.get () in
+  (**) assert(modifies (lbufferOpt_loc hs.k_xy |+| lbufferOpt_loc hs.k_auth_I
+              |+| lbufferOpt_loc hs.th2 |+| lbufferOpt_loc hs.prk2e) h0 h4);
+
+  ()
+
+#pop-options
+
+(*----------------- Responder's side*)
+val responder_send_msg2_set_up:
+  kcs: supportedKemCipherSuite
+  -> rs: party_state_m kcs
+  -> hs: handshake_state_m kcs
+  -> msg1: message1 kcs
+  -> msg2: message2 kcs
+  -> ST.Stack unit
+  (requires fun h0 ->
+    is_valid_handshake_state_m h0 hs
+    /\ is_valid_party_state_m h0 rs
+    /\ is_valid_message1 h0 msg1 /\ is_legit_message1 h0 msg1
+    /\ is_valid_message2 h0 msg2
+    /\ live h0 kem_state /\ live h0 entropy_p
+
+    // Disjointness
+    /\ handshake_state_m_disjoint_to_party_state hs rs
+    /\ handshake_state_m_disjoint_to_msg1 hs msg1
+    /\ handshake_state_m_disjoint_to_msg2 hs msg2
+    /\ handshake_state_m_disjoint_to_lbuffer hs kem_state
+    /\ handshake_state_m_disjoint_to_lbuffer hs entropy_p
+    /\ party_state_disjoint_to_msg1 rs msg1
+    /\ party_state_disjoint_to_msg2 rs msg2
+    /\ party_state_disjoint_to_lbuffer rs kem_state
+    /\ party_state_disjoint_to_lbuffer rs entropy_p
+    /\ message1_disjoint_to_lbuffer msg1 kem_state
+    /\ message1_disjoint_to_lbuffer msg1 entropy_p
+    /\ message2_disjoint_to_lbuffer msg2 kem_state
+    /\ message2_disjoint_to_lbuffer msg2 entropy_p
+    /\ message2_disjoint_to_msg1 msg2 msg1
+    /\ disjoint kem_state entropy_p
+  )
+  (ensures fun h0 _ h1 ->
+    let modified_locs
+      = loc kem_state |+| loc entropy_p |+|
+      lbufferOpt_loc hs.k_xy |+| loc msg2.ct_y
+      |+| loc msg2.ct_auth_I |+| lbufferOpt_loc hs.k_auth_I
+      |+| lbufferOpt_loc hs.th2
+      |+| lbufferOpt_loc hs.prk2e |+| lbufferOpt_loc hs.prk3e2m in
+
+    modifies modified_locs h0 h1
+    /\ is_valid_handshake_state_m h1 hs
+    /\ is_valid_party_state_m h1 rs
+    /\ is_valid_message1 h0 msg1 /\ is_valid_message2 h0 msg2
+
+  )
+
+#push-options "--z3refresh --z3rlimit 60 --max_fuel 4 --max_ifuel 4"
+let responder_send_msg2_set_up_uti (kcs: supportedKemCipherSuite)
+  (rs: party_state_m kcs) (hs: handshake_state_m kcs)
+  (msg1: message1 kcs) (msg2: message2 kcs)
+  : ST.Stack unit
+  (requires fun h0 ->
+    is_valid_handshake_state_m h0 hs
+    /\ is_valid_party_state_m h0 rs
+    /\ is_valid_message1 h0 msg1 /\ is_legit_message1 h0 msg1
+    /\ is_valid_message2 h0 msg2
+    /\ live h0 kem_state /\ live h0 entropy_p
+
+    // Disjointness
+    /\ handshake_state_m_disjoint_to_party_state hs rs
+    /\ handshake_state_m_disjoint_to_msg1 hs msg1
+    /\ handshake_state_m_disjoint_to_msg2 hs msg2
+    /\ handshake_state_m_disjoint_to_lbuffer hs kem_state
+    /\ handshake_state_m_disjoint_to_lbuffer hs entropy_p
+    /\ party_state_disjoint_to_msg1 rs msg1
+    /\ party_state_disjoint_to_msg2 rs msg2
+    /\ party_state_disjoint_to_lbuffer rs kem_state
+    /\ party_state_disjoint_to_lbuffer rs entropy_p
+    /\ message1_disjoint_to_lbuffer msg1 kem_state
+    /\ message1_disjoint_to_lbuffer msg1 entropy_p
+    /\ message2_disjoint_to_lbuffer msg2 kem_state
+    /\ message2_disjoint_to_lbuffer msg2 entropy_p
+    /\ message2_disjoint_to_msg1 msg2 msg1
+    /\ disjoint kem_state entropy_p
+  )
+  (ensures fun h0 _ h1 ->
+    let modified_locs = loc kem_state |+| loc entropy_p
+              |+| lbufferOpt_loc hs.k_xy |+| loc msg2.ct_y
+              |+| lbufferOpt_loc hs.k_auth_I |+| loc msg2.ct_auth_I
+              |+| lbufferOpt_loc hs.th2 |+| lbufferOpt_loc hs.prk2e in
+
+    modifies modified_locs h0 h1
+    /\ is_valid_handshake_state_m h1 hs
+    /\ is_valid_party_state_m h1 rs
+    /\ is_valid_message1 h0 msg1 /\ is_valid_message2 h0 msg2
+  )
+  = (**) let h0 = ST.get () in
+  
+  // ecnaps pk_x -> ct_y, k_xy
+  kem_encaps kcs msg1.pk_x msg2.ct_y hs.k_xy.value;
+  lbufferOpt_set_Some hs.k_xy; // set Some for k_xy
+  (**) let h1 = ST.get () in
+  (**) assert(modifies (loc kem_state |+| loc entropy_p
+              |+| lbufferOpt_loc hs.k_xy |+| loc msg2.ct_y) h0 h1);
+
+  // encaps pk_I -> ct_auth_I, k_auth_I
+  let pk_I = rs.remote_static_kem_pub_key in
+  kem_encaps kcs pk_I msg2.ct_auth_I hs.k_auth_I.value;
+  lbufferOpt_set_Some hs.k_auth_I; // set Some for k_auth_I
+  (**) let h2 = ST.get () in
+  (**) assert(modifies (loc kem_state |+| loc entropy_p
+              |+| lbufferOpt_loc hs.k_xy |+| loc msg2.ct_y
+              |+| lbufferOpt_loc hs.k_auth_I |+| loc msg2.ct_auth_I) h0 h2);
+
+  // derive TH2
+  compute_th2 #kcs msg2.ct_y hs.k_auth_I.value msg1 hs.th2.value;
+  lbufferOpt_set_Some hs.th2; // set Some for th2
+  (**) let h3 = ST.get () in
+  (**) assert(modifies (loc kem_state |+| loc entropy_p
+              |+| lbufferOpt_loc hs.k_xy |+| loc msg2.ct_y
+              |+| lbufferOpt_loc hs.k_auth_I |+| loc msg2.ct_auth_I
+              |+| lbufferOpt_loc hs.th2) h0 h3);
+
+  // derive PRK2e
+  extract_prk2e #kcs hs.prk1e hs.th2.value hs.k_xy.value hs.prk2e.value;
+  lbufferOpt_set_Some hs.prk2e; // set Some for prk2e
+  ()
+
+
+let responder_send_msg2_set_up kcs rs hs msg1 msg2
+  = (**) let h0 = ST.get () in
+  ST.push_frame ();
+
+  responder_send_msg2_set_up_uti kcs rs hs msg1 msg2;
+
+  // derive SAlT3e2m
+  let salt3e2m = create (hash_size_t kcs) (u8 0) in
+  expand_salt #kcs SpecKS.info_label_salt3e2m hs.prk2e.value hs.th2.value salt3e2m;
+
+  // derive PRK3e2m
+  extract_prk3e2m #kcs salt3e2m hs.k_auth_R hs.prk3e2m.value;
+  lbufferOpt_set_Some hs.prk3e2m; // set Some for prk3e2m
+
+  ST.pop_frame ();
+  (**) let h_final = ST.get () in
+  (**) assert(modifies (loc kem_state |+| loc entropy_p
+              |+| lbufferOpt_loc hs.k_xy |+| loc msg2.ct_y
+              |+| lbufferOpt_loc hs.k_auth_I |+| loc msg2.ct_auth_I
+              |+| lbufferOpt_loc hs.th2
+              |+| lbufferOpt_loc hs.prk2e |+| lbufferOpt_loc hs.prk3e2m) h0 h_final);
+  ()
+
+#pop-options
+
+val responder_construct_msg2:
+  kcs: supportedKemCipherSuite
+  -> rs: party_state_m kcs
+  -> hs: handshake_state_m kcs
+  -> msg2: message2 kcs
+  -> ST.Stack c_response
+  (requires fun h0 ->
+    is_valid_handshake_state_m h0 hs
+    /\ is_valid_party_state_m h0 rs
+    /\ is_valid_message2 h0 msg2
+    /\ live h0 entropy_p
+
+    // Disjointness
+    /\ handshake_state_m_disjoint_to_party_state hs rs
+    /\ handshake_state_m_disjoint_to_msg2 hs msg2
+    /\ handshake_state_m_disjoint_to_lbuffer hs entropy_p
+    /\ party_state_disjoint_to_msg2 rs msg2
+    /\ party_state_disjoint_to_lbuffer rs entropy_p
+    /\ message2_disjoint_to_lbuffer msg2 entropy_p
+  )
+  (ensures fun h0 res h1 ->
+    True
+    // (match res with
+    //   | TypeEdhoc.CUnsupportedAlgorithmOrInvalidConfig -> modifies0 h0 h1
+    //   | TypeEdhoc.CSuccess -> modifies1 msg2.c2 h0 h1
+    //   | _ -> False)
+    // /\ is_valid_handshake_state_m h1 hs
+    // /\ is_valid_party_state_m h1 rs
+    // /\ is_valid_message2 h1 msg2
+  )
+
+#push-options "--z3refresh --z3rlimit 60 --max_fuel 4 --max_ifuel 4"
+let responder_construct_msg2 kcs rs hs msg2
+  = (**) let h0 = ST.get () in
+  ST.push_frame ();
+
+  // randomly generate connection ID C_R
+  let c_R = create (size SpecParser.c_id_size) (u8 0) in
+  crypto_random c_R (size SpecParser.c_id_size);
+  // get credential cred_R
+  let cred_R = create (size SpecParser.cred_size) (u8 0) in
+  copy cred_R rs.id_cred;
+  (**) let h1 = ST.get() in
+
+  // construct context2
+  let ctx2: context2 kcs = {
+    c_r = c_R;
+    id_cred_r = rs.id_cred;
+    th2 = hs.th2.value;
+    cred_r = cred_R;
+  } in
+
+  // let res = responder_construct_msg2_uti #kcs hs ctx2 msg2.c2 in
+
+  ST.pop_frame ();
+  (**) let h_final = ST.get () in
+  // (**) assert(
+  //   match res with
+  //     | TypeEdhoc.CUnsupportedAlgorithmOrInvalidConfig -> modifies0 h0 h_final
+  //     | TypeEdhoc.CSuccess -> modifies1 msg2.c2 h0 h_final
+  // );
+  // (**) assert(is_valid_handshake_state_m h_final hs
+  //     /\ is_valid_party_state_m h_final rs
+  //     /\ is_valid_message2 h_final msg2
+  // );
+  // res
+  TypeEdhoc.CSuccess
+
+#pop-options
